src/Crypto/RSAEncryption.dfy
@@ -1,80 +1,170 @@
 include "../StandardLibrary/StandardLibrary.dfy"
 
 module {:extern "RSAEncryption"} RSAEncryptionDef {
-    import opened StandardLibrary
-    import opened UInt = StandardLibrary.UInt
+  import opened StandardLibrary
+  import opened UInt = StandardLibrary.UInt
 
-    datatype {:extern "PaddingMode"} PaddingMode = PKCS1 | OAEP_SHA1 | OAEP_SHA256 | OAEP_SHA384 | OAEP_SHA512
+  datatype {:extern "PaddingMode"} PaddingMode = PKCS1 | OAEP_SHA1 | OAEP_SHA256 | OAEP_SHA384 | OAEP_SHA512
 
-    // The smallest ciphertext length is defined using PKCS1, where messageLength <= k - 11 and k represents the length
-    // in octets (bytes) of the modulus n. This means that the minimum possible strength in bits can be calculated as:
-    // (strength + 7) / 8 - 11 == 0 ==> min strength == 81 in this scenario (where messageLength == 0). In practice,
-    // this number should be much higher (at least 1024 or, better, 2048).
-    // TODO: Determine if we want to enforce a min value of 2048 bits as the min strength (requires updating the spec)
-    newtype {:nativeType "int"} StrengthBits = x | 81 <= x < (0x8000_0000) witness 81
+  // The smallest ciphertext length is defined using PKCS1, where messageLength <= k - 11 and k represents the strength,
+  // defined as the length in octets (bytes) of the modulus n. This means that the minimum possible strength in bits
+  // can be calculated as: (strength + 7) / 8 - 11 == 0 ==> min strength == 81 in this scenario
+  // (where messageLength == 0). In practice, this number should be much higher (at least 1024 or, better, 2048).
+  // TODO: Determine if we want to enforce a min value of 2048 bits as the min strength (requires updating the spec)
+  newtype {:nativeType "int"} StrengthBits = x | 81 <= x < (0x8000_0000) witness 81
 
-    // Represents the length in octets (bytes) of the hash function output
-    const SHA1_HASH_BYTES := 20
-    const SHA256_HASH_BYTES := 32
-    const SHA384_HASH_BYTES := 48
-    const SHA512_HASH_BYTES := 64
-
-    // GetBytes converts the given number of bits to the octet (byte) size that can include all bits
-    function method GetBytes(bits : nat) : nat {
-      (bits + 7) / 8
-    }
-
-    // MinStrengthBytes represents the minimum strength (in bytes) required for a given padding
-    function method MinStrengthBytes(padding : PaddingMode) : nat {
-      match padding {
-        // 0 = k - 11 ==> k = 11
-        case PKCS1 => 11
-        // 0 = k - 2 * hashLengthBytes - 2 ==> k = 2 + 2 * hashLengthBytes
-        case OAEP_SHA1 => 2 * SHA1_HASH_BYTES + 2
-        case OAEP_SHA256 => 2 * SHA256_HASH_BYTES + 2
-        case OAEP_SHA384 => 2 * SHA384_HASH_BYTES + 2
-        case OAEP_SHA512 => 2 * SHA512_HASH_BYTES + 2
-        }
-    }
-
-    // MaxPlaintextBytes represents the maximum size (in bytes) that the plaintext data can be for a given strength
-    // (in bits) and padding mode
-    function method MaxPlaintextBytes(padding : PaddingMode, strength : nat) : nat
-      requires GetBytes(strength) >= MinStrengthBytes(padding)
+  // This trait represents the parent for RSA public and private keys
+  trait {:termination false} Key {
+    ghost var Repr : set<object>
+    ghost const strength : StrengthBits
+    ghost const padding : PaddingMode
+    const pem : seq<uint8>
+    predicate Valid() reads this, Repr
     {
-      match padding {
-        // mLen <= k - 11
-        case PKCS1 => GetBytes(strength) - 11
-        // Per  mLen <= k - 2 * hashLengthBytes - 2
-        case OAEP_SHA1 => GetBytes(strength) - 2 * SHA1_HASH_BYTES - 2
-        case OAEP_SHA256 => GetBytes(strength) - 2 * SHA256_HASH_BYTES - 2
-        case OAEP_SHA384 => GetBytes(strength) - 2 * SHA384_HASH_BYTES - 2
-        case OAEP_SHA512 => GetBytes(strength) - 2 * SHA512_HASH_BYTES - 2
-        }
+      Repr == {this} &&
+      |pem| > 0 &&
+      GetBytes(strength) >= MinStrengthBytes(padding)
     }
+  }
 
-    // The full extern name needs to be specified here (and below) to prevent conflicts when resolving the extern
-    method {:extern "RSAEncryption.RSA", "GenerateKeyPair"} GenerateKeyPair(strength : StrengthBits, padding: PaddingMode)
-        returns (publicKey : seq<uint8>, privateKey : seq<uint8>)
-      requires GetBytes(strength as nat) >= MinStrengthBytes(padding)
-      ensures |publicKey| > 0
-      ensures |privateKey| > 0
-      //ensures |privateKey.pem| > 0
-      //ensures privateKey.strength = strength
+  // PrivateKey represents an extension of Key for RSA private keys to aid with type safety
+  class PrivateKey extends Key {
+    constructor(pem: seq<uint8>, strength: StrengthBits, padding: PaddingMode)
+    requires |pem| > 0
+    requires GetBytes(strength) >= MinStrengthBytes(padding)
+    ensures this.pem == pem
+    ensures this.strength == strength
+    ensures this.padding == padding
+    ensures Valid()
+    {
+      this.pem := pem;
+      this.strength := strength;
+      this.padding := padding;
+      Repr := {this};
+    }
+  }
 
-    method {:extern "RSAEncryption.RSA", "Decrypt"} Decrypt(padding : PaddingMode, privateKey : seq<uint8>,
-                                                            cipherText : seq<uint8>)
-        returns (res : Result<seq<uint8>>)
-      requires |privateKey| > 0
-      // requires GetBytes(privateKey.strength) >= |cipherText|
-      requires |cipherText| > 0
-      // TODO: Validate that the cipherText length == k, the length in octets of the modulus n
+  // PublicKey represents an extension of Key for RSA public keys to aid with type safety
+  class PublicKey extends Key {
+    constructor(pem: seq<uint8>, strength: StrengthBits, padding: PaddingMode)
+    requires |pem| > 0
+    requires GetBytes(strength) >= MinStrengthBytes(padding)
+    ensures this.pem == pem
+    ensures this.strength == strength
+    ensures this.padding == padding
+    ensures Valid()
+    {
+      this.pem := pem;
+      this.strength := strength;
+      this.padding := padding;
+      Repr := {this};
+    }
+  }
 
-    method {:extern "RSAEncryption.RSA", "Encrypt"} Encrypt(padding: PaddingMode, publicKey : seq<uint8>,
-                                                            plaintextData : seq<uint8>)
-        returns (res : Result<seq<uint8>>)
-      requires |publicKey| > 0
-      requires |plaintextData| > 0
-     // requires |plaintextData| <= MaxPlaintextBytes(publicKey.strength, padding)
-      // TODO: Validate that the plaintextData length <= MaxPlaintextBytes(padding, modulus from public key)
+  // Represents the length in octets (bytes) of the hash function output
+  const SHA1_HASH_BYTES := 20
+  const SHA256_HASH_BYTES := 32
+  const SHA384_HASH_BYTES := 48
+  const SHA512_HASH_BYTES := 64
+
+  // GetBytes converts a bit strength into the octet (byte) size that can include all bits
+  function method GetBytes(bits : StrengthBits) : nat {
+    (bits as nat + 7) / 8
+  }
+
+  // MinStrengthBytes represents the minimum strength (in bytes) required for a given padding
+  function method MinStrengthBytes(padding : PaddingMode) : nat {
+    match padding {
+      // 0 = k - 11 ==> k = 11
+      case PKCS1 => 11
+      // 0 = k - 2 * hashLengthBytes - 2 ==> k = 2 + 2 * hashLengthBytes
+      case OAEP_SHA1 => 2 * SHA1_HASH_BYTES + 2
+      case OAEP_SHA256 => 2 * SHA256_HASH_BYTES + 2
+      case OAEP_SHA384 => 2 * SHA384_HASH_BYTES + 2
+      case OAEP_SHA512 => 2 * SHA512_HASH_BYTES + 2
+      }
+  }
+
+  // MaxPlaintextBytes represents the maximum size (in bytes) that the plaintext data can be for a given strength
+  // (in bits) and padding mode
+  function method MaxPlaintextBytes(padding : PaddingMode, strength : StrengthBits) : nat
+    requires GetBytes(strength) >= MinStrengthBytes(padding)
+  {
+    match padding {
+      // mLen <= k - 11
+      case PKCS1 => GetBytes(strength) - 11
+      // Per  mLen <= k - 2 * hashLengthBytes - 2
+      case OAEP_SHA1 => GetBytes(strength) - 2 * SHA1_HASH_BYTES - 2
+      case OAEP_SHA256 => GetBytes(strength) - 2 * SHA256_HASH_BYTES - 2
+      case OAEP_SHA384 => GetBytes(strength) - 2 * SHA384_HASH_BYTES - 2
+      case OAEP_SHA512 => GetBytes(strength) - 2 * SHA512_HASH_BYTES - 2
+      }
+  }
+
+  method GenerateKeyPair(strength : StrengthBits, padding: PaddingMode)
+      returns (publicKey : PublicKey, privateKey : PrivateKey)
+    requires GetBytes(strength) >= MinStrengthBytes(padding)
+    ensures privateKey.Valid()
+    ensures privateKey.strength == strength
+    ensures privateKey.padding == padding
+    ensures publicKey.Valid()
+    ensures publicKey.strength == strength
+    ensures publicKey.padding == padding
+    ensures GetBytes(publicKey.strength) >= MinStrengthBytes(publicKey.padding)
+    ensures GetBytes(privateKey.strength) >= MinStrengthBytes(privateKey.padding)
+  {
+    var pemPublic, pemPrivate := GenerateKeyPairExtern(strength, padding);
+    privateKey := new PrivateKey(pemPrivate, strength, padding);
+    publicKey := new PublicKey(pemPublic, strength, padding);
+  }
+
+  method Decrypt(padding : PaddingMode, privateKey : PrivateKey, cipherText : seq<uint8>) returns (res : Result<seq<uint8>>)
+    requires privateKey.Valid()
+    requires 0 < |cipherText|
+    // TODO: Is there a way to enable this without making strength non-ghost for the RawRSAKeyring
+    // requires|cipherText| <= GetBytes(privateKey.strength)
+    requires padding == privateKey.padding
+    ensures privateKey.Valid()
+  {
+    res := DecryptExtern(padding, privateKey.pem, cipherText);
+  }
+
+  method Encrypt(padding: PaddingMode, publicKey : PublicKey, plaintextData : seq<uint8>) returns (res : Result<seq<uint8>>)
+    requires publicKey.Valid()
+    requires GetBytes(publicKey.strength) >= MinStrengthBytes(padding)
+    requires 0 < |plaintextData|
+    // TODO: Is there a way to enable this without making strength non-ghost for the RawRSAKeyring
+    // requires |plaintextData| <= MaxPlaintextBytes(padding, publicKey.strength)
+    requires padding == publicKey.padding
+    ensures publicKey.Valid()
+  {
+    res := EncryptExtern(padding, publicKey.pem, plaintextData);
+  }
+
+  // The full extern name needs to be specified here (and below) to prevent conflicts when resolving the extern
+  // Note: Customers should call GenerateKeyPair instead of GenerateKeyPairExtern to ensure type safety and additional
+  // verification
+  method {:extern "RSAEncryption.RSA", "GenerateKeyPairExtern"} GenerateKeyPairExtern(strength : StrengthBits,
+                                                                                      padding: PaddingMode)
+      returns (publicKey : seq<uint8>, privateKey : seq<uint8>)
+    requires GetBytes(strength) >= MinStrengthBytes(padding)
+    ensures |publicKey| > 0
+    ensures |privateKey| > 0
+
+  // Note: Customers should call Decrypt instead of DecryptExtern to ensure type safety and additional
+  // verification
+  method {:extern "RSAEncryption.RSA", "DecryptExtern"} DecryptExtern(padding : PaddingMode, privateKey : seq<uint8>,
+                                                                      cipherText : seq<uint8>)
+      returns (res : Result<seq<uint8>>)
+    requires |privateKey| > 0
+    requires |cipherText| > 0
+
+
+  // Note: Customers should call Encrypt instead of EncryptExtern to ensure type safety and additional
+  // verification
+  method {:extern "RSAEncryption.RSA", "EncryptExtern"} EncryptExtern(padding: PaddingMode, publicKey : seq<uint8>,
+                                                                      plaintextData : seq<uint8>)
+      returns (res : Result<seq<uint8>>)
+    requires |publicKey| > 0
+    requires |plaintextData| > 0
 }
